feat: poset `IGame` (#63)

CombinatorialGames/IGame/Concrete.lean
@@ -4,11 +4,12 @@ Released under Apache 2.0 license as described in the file LICENSE.
 Authors: Violeta Hernández Palacios
 -/
 import CombinatorialGames.IGame.IGame
+import CombinatorialGames.IGame.Impartial
 
 /-!
 # Combinatorial games from a type of states
 
-A "concrete" game is a type of states endowed with well-founded subsequence relations for the
+A "concrete" game is a type of states endowed with well-founded move relations for the
 left and right players. This is often a more convenient representation for a game, which can then be
 used to define a `IGame`.
 -/
@@ -19,45 +20,45 @@ open IGame
 
 variable {α : Type*}
 
-/-- A "concrete" game is a type of states endowed with well-founded subsequence relations for the
+/-- A "concrete" game is a type of states endowed with well-founded move relations for the
 left and right players. -/
 class ConcreteGame (α : Type*) where
-  /-- The subsequence relation for the left player. -/
-  subsequentL : α → α → Prop
-  /-- The subsequence relation for the right player. -/
-  subsequentR : α → α → Prop
-  /-- The subsequence relation is well-founded. -/
-  isWellFounded_subsequent : IsWellFounded α fun a b ↦ subsequentL a b ∨ subsequentR a b
+  /-- The move relation for the left player. -/
+  relLeft : α → α → Prop
+  /-- The move relation for the right player. -/
+  relRight : α → α → Prop
+  /-- The move relation is well-founded. -/
+  isWellFounded_rel : IsWellFounded α fun a b ↦ relLeft a b ∨ relRight a b
 
 namespace ConcreteGame
 variable [ConcreteGame α]
 
-local infix:50 " ≺ₗ " => subsequentL
-local infix:50 " ≺ᵣ " => subsequentR
-attribute [instance] isWellFounded_subsequent
+local infix:50 " ≺ₗ " => relLeft
+local infix:50 " ≺ᵣ " => relRight
+attribute [instance] isWellFounded_rel
 
-theorem subrelation_subsequentL :
-    Subrelation subsequentL fun a b : α ↦ subsequentL a b ∨ subsequentR a b :=
+theorem subrelation_relLeft :
+    Subrelation relLeft fun a b : α ↦ relLeft a b ∨ relRight a b :=
   Or.inl
 
-theorem subrelation_subsequentR :
-    Subrelation subsequentR fun a b : α ↦ subsequentL a b ∨ subsequentR a b :=
+theorem subrelation_relRight :
+    Subrelation relRight fun a b : α ↦ relLeft a b ∨ relRight a b :=
   Or.inr
 
-instance [ConcreteGame α] : IsWellFounded α subsequentL := subrelation_subsequentL.isWellFounded
-instance [ConcreteGame α] : IsWellFounded α subsequentR := subrelation_subsequentR.isWellFounded
+instance [ConcreteGame α] : IsWellFounded α relLeft := subrelation_relLeft.isWellFounded
+instance [ConcreteGame α] : IsWellFounded α relRight := subrelation_relRight.isWellFounded
 
 /-- Defines a concrete game from a single relation, to be used for both players. -/
 def ofImpartial (r : α → α → Prop) [h : IsWellFounded α r] : ConcreteGame α where
-  subsequentL := r
-  subsequentR := r
-  isWellFounded_subsequent := by convert h; rw [or_self]
+  relLeft := r
+  relRight := r
+  isWellFounded_rel := by convert h; rw [or_self]
 
 /-- Turns a state of a `ConcreteGame` into an `IGame`. -/
 def toIGame (a : α) : IGame :=
   {.range fun b : {b // b ≺ₗ a} ↦ toIGame b |
     .range fun b : {b // b ≺ᵣ a} ↦ toIGame b}ᴵ
-termination_by isWellFounded_subsequent.wf.wrap a
+termination_by isWellFounded_rel.wf.wrap a
 decreasing_by all_goals aesop
 
 theorem toIGame_def (a : α) : toIGame a = {toIGame '' {b | b ≺ₗ a} | toIGame '' {b | b ≺ᵣ a}}ᴵ := by
@@ -71,7 +72,17 @@ theorem leftMoves_toIGame (a : α) : (toIGame a).leftMoves = toIGame '' {b | b �
 theorem rightMoves_toIGame (a : α) : (toIGame a).rightMoves = toIGame '' {b | b ≺ᵣ a} := by
   rw [toIGame_def, rightMoves_ofSets]
 
-theorem neg_toIGame (h : subsequentL (α := α) = subsequentR) (a : α) : -toIGame a = toIGame a := by
+theorem mem_leftMoves_toIGame_of_relLeft {a b : α} (hab : b ≺ₗ a) :
+    toIGame b ∈ (toIGame a).leftMoves := by
+  rw [leftMoves_toIGame]
+  exact ⟨b, hab, rfl⟩
+
+theorem mem_rightMoves_toIGame_of_relRight {a b : α} (hab : b ≺ᵣ a) :
+    toIGame b ∈ (toIGame a).rightMoves := by
+  rw [rightMoves_toIGame]
+  exact ⟨b, hab, rfl⟩
+
+theorem neg_toIGame (h : relLeft (α := α) = relRight) (a : α) : -toIGame a = toIGame a := by
   ext
   all_goals
     simp only [leftMoves_neg, rightMoves_neg, rightMoves_toIGame, Set.mem_neg, Set.mem_image,
@@ -80,24 +91,19 @@ theorem neg_toIGame (h : subsequentL (α := α) = subsequentR) (a : α) : -toIGa
     rw [and_congr_right_iff]
     intros
     rw [← neg_eq_iff_eq_neg, neg_toIGame h]
-termination_by isWellFounded_subsequent.wf.wrap a
+termination_by isWellFounded_rel.wf.wrap a
 decreasing_by all_goals aesop
 
--- TODO: port once we have impartial games
-
-/-
-theorem impartial_toPGame (h : subsequentL (α := α) = subsequentR) (a : α) :
-    Impartial (toPGame a) := by
-  rw [impartial_def, neg_toPGame h]
-  refine ⟨.rfl, fun i ↦ ?_, fun i ↦ ?_⟩
-  · rw [moveLeft_toPGame]
-    have := subrelation_subsequentL <| toLeftMovesToPGame_symm_prop i
-    exact impartial_toPGame h _
-  · rw [moveRight_toPGame]
-    have := subrelation_subsequentR <| toRightMovesToPGame_symm_prop i
-    exact impartial_toPGame h _
-termination_by isWellFounded_subsequent.wf.wrap a
--/
+theorem impartial_toIGame (h : relLeft (α := α) = relRight) (a : α) :
+    (toIGame a).Impartial := by
+  rw [impartial_def, neg_toIGame h, leftMoves_toIGame, rightMoves_toIGame]
+  refine ⟨.rfl, fun i hi ↦ ?_, fun i hi ↦ ?_⟩
+  all_goals rw [← hi.choose_spec.2]
+  · have := subrelation_relLeft <| hi.choose_spec.1
+    exact impartial_toIGame h _
+  · have := subrelation_relRight <| hi.choose_spec.1
+    exact impartial_toIGame h _
+termination_by isWellFounded_rel.wf.wrap a
 
 end ConcreteGame
 end
